feat: add a typed IR for NKI and its typing rules

KLR/NKI/Types.lean
@@ -3,161 +3,359 @@ Copyright (c) 2025 Amazon.com, Inc. or its affiliates. All Rights Reserved.
 Released under Apache 2.0 license as described in the file LICENSE.
 Authors: Paul Mure
 -/
+import KLR.NKI.Basic
 import KLR.Core.Operators
-
-/--
-Type-level membership with notation `s ∋ a : Type` where `a : α` and `s : γ`.
-Since `α` is an `outParam`, the container type `γ` determines the element type.
-
-This differs from the standard library `Membership` class because our `mem` function
-returns a `Type` instead of a `Prop`, making it suitable for dependent De Bruijn indexing.
--/
-class Mem (α : outParam (Type u)) (γ : Type v) where
-  /-- The membership relation `s ∋ α : Type*` where `a : α` and `s : γ`. -/
-  mem : γ → α → Type (max u v)
-infix:60 " ∋ " => Mem.mem
-
-/--
-Dependent list membership for De Bruijn indexing.
--/
-inductive List.Member {α : Type u} : List α → α → Type u
-  | head {a : α} {as : List α} : List.Member (a::as) a
-  | tail {bs : List α} {a b : α} : List.Member bs b → List.Member (a::bs) b
-
-instance instMemList {α} : Mem α (List α) where
-  mem := List.Member
+import KLR.Compile.Pass
 
 namespace KLR.NKI.Types
 
-/-- The kinds of types in our type system. -/
+/-!
+# NKI's Type System
+-/
+
 inductive Kind
-  /-- Dimension values (natural numbers) -/
   | dim
-  /-- Tensor shapes (lists of dimensions) -/
   | shape
-  /-- Regular types -/
-  | type
-  /--
-  Type-level propositions for constraint solving.
+  | typ
+deriving DecidableEq, BEq, Repr
 
-  These represent assertions about types that users write in function preambles.
-  The type checker runs a solver to verify their satisfiability, rather than
-  requiring explicit proof construction like in traditional theorem provers.
-  They act as type constraints for the solver to handle automatically.
-
-  The goal here is to have users write python `assert`s and parse them
-  into types by reflecting python expressions up to the NKI type level.
-  -/
-  | prop
-scoped notation "⋆" => Kind.type
-
-abbrev TypCtx := List Kind
-
-/-- Context extension: `Φ,, κ ≡ κ :: Φ`. -/
-scoped notation:70 Φ:70 ",, " κ:71 => @List.cons Kind κ Φ
-
-/-- Primitive types in the NKI type system. -/
 inductive Prim
   | none
   | bool
   | int
   | float
   | string
-  /--
-  Data type wrapper for tensor indexing.
-  Currently not directly constructible in the AST.
-  -/
-  | dtype (dt : Core.Dtype) : Prim
+  | dtype (dt : Core.Dtype)
+deriving DecidableEq, BEq
 
-mutual
-
-/-- Types indexed by context and kind. -/
-inductive Types : TypCtx → Kind → Type
+inductive Typ
   /-- Type variable reference -/
-  | var {Φ : TypCtx} {κ : Kind} (mem : Φ ∋ κ) : Types Φ κ
+  | var (idx : Nat)
   /-- Polymorphic universal quantification -/
-  | pi {Φ : TypCtx} (κ : Kind) (typ : Types (Φ,, κ) ⋆) : Types Φ ⋆
+  | pi (κ : Kind) (typ : Typ)
   /-- Primitive types -/
-  | prim {Φ : TypCtx} (p : Prim) : Types Φ ⋆
-  /-- Tuple types -/
-  | tuple {Φ : TypCtx} (ts : TList Φ ⋆) : Types Φ ⋆
+  | prim (p : Prim)
   /-- Function types -/
-  | func {Φ : TypCtx} (dom ran : Types Φ ⋆) : Types Φ ⋆
+  | func (dom ran : Typ)
   /-- Dimension literals -/
-  | dim {Φ : TypCtx} (n : Nat) : Types Φ .dim
+  | dim (n : Nat)
   /-- Tensor shapes -/
-  | shape {Φ : TypCtx} (dims : TList Φ .dim) : Types Φ .shape
+  | shape (dims : List Typ)
   /-- Tensor types with shape and data type -/
-  | tensor {Φ : TypCtx} (shape : Types Φ .shape) (dt : Core.Dtype) : Types Φ ⋆
+  | tensor (shape : Typ) (dt : Core.Dtype)
   -- Dimension operations
   /-- Dimension addition -/
-  | dimAdd {Φ : TypCtx} (x y : Types Φ .dim) : Types Φ .dim
+  | dimAdd (x y : Typ)
   -- Shape operations
   /-- Shape concatenation -/
-  | shapeAppend {Φ : TypCtx} (s1 s2 : Types Φ .shape) : Types Φ .shape
-  -- Propositions
-  /-- Dimension equality constraint -/
-  | dimEq {Φ : TypCtx} (x y : Types Φ .dim) : Types Φ .prop
+  | shapeAppend (s1 s2 : Typ)
+  /-- The tail of a shape -/
+  | shapeTail (s : Typ)
+deriving BEq
 
-/-- Homogeneous lists of types with the same kind. -/
-inductive TList : TypCtx → Kind → Type
-  | nil {Φ κ} : TList Φ κ
-  | cons {Φ κ} (hd : Types Φ κ) (tl : TList Φ κ) : TList Φ κ
+def Kind.toString : Kind → String
+  | .dim => "dim"
+  | .shape => "shape"
+  | .typ => "⋆"
 
-end
+instance Kind.instToStringKind : ToString Kind where
+  toString := Kind.toString
+
+instance Kind.instReprKind : Repr Kind where
+  reprPrec k _ := k.toString
+
+def Prim.toString : Prim → String
+  | .none => "none"
+  | .bool => "bool"
+  | .int => "int"
+  | .float => "float"
+  | .string => "string"
+  | .dtype dt => dt.toString
+
+instance Prim.instToStringPrim : ToString Prim where
+  toString := Prim.toString
+
+instance Prim.instReprPrim : Repr Prim where
+  reprPrec p _ := p.toString
+
+def Typ.reprPrec (t : Typ) (n : Nat) : Std.Format :=
+  match t with
+  | .var idx => s!"v_{idx}"
+  | .pi κ typ => s!"Π {κ} ⇒ {typ.reprPrec 1000}"
+  | .prim p => p.toString
+  | .func dom ran =>
+    let fmt := s!"{dom.reprPrec n} ⟶ {ran.reprPrec (n + 1)}"
+    if n > 10 then
+      fmt
+    else
+      Std.Format.paren fmt
+  | .dim n => s!"dim({n})"
+  | .shape dims =>
+    let dims := Std.Format.join (dims.map fun t => (Typ.reprPrec t 1000) ++ ", ")
+    s!"shape[{dims}]"
+  | .tensor sh dt =>
+    s!"tensor[{sh.reprPrec 1000}, {dt}]"
+  | .dimAdd x y =>
+    let fmt := s!"{x.reprPrec (n + 1)} + {y.reprPrec n}"
+    if n > 50 then
+      fmt
+    else
+      Std.Format.paren fmt
+  | .shapeAppend s1 s2 =>
+    let fmt := s!"{s1.reprPrec (n + 1)} ++ {s2.reprPrec n}"
+    if n > 50 then
+      fmt
+    else
+      Std.Format.paren fmt
+  | .shapeTail t =>
+    s!"({t.reprPrec 1000}).tail"
+
+instance Typ.instReprTyp : Repr Typ where
+  reprPrec :=  Typ.reprPrec
 
 /-!
-# Type notation and syntax
+# Some syntax for writing down types
 -/
 
-/-- `Φ ⊢⋆ κ` denotes a type of kind `κ` under type context `Φ`. -/
-scoped infix:50 " ⊢⋆ " => Types
+scoped notation "⋆" => Kind.typ
 
-scoped infixr:55 " → " => Types.func
-
-/-- Most recently bound variable (De Bruijn index 0) -/
-scoped notation "v0" => Types.var List.Member.head
-/-- Second most recently bound variable (De Bruijn index 1) -/
-scoped notation "v1" => Types.var <| List.Member.tail List.Member.head
-/-- Third most recently bound variable (De Bruijn index 2) -/
-scoped notation "v2" => Types.var <| List.Member.tail <| List.Member.tail List.Member.head
-/-- Fourth most recently bound variable (De Bruijn index 3) -/
-scoped notation "v3" => Types.var <| List.Member.tail <| List.Member.tail <| List.Member.tail List.Member.head
+infixr:10 " ⟶ " => Typ.func
 
 /--
 `Π κ, ι ⇒ body` binds kinds `κ` and `ι` in `body` using `Types.pi`.
-Variables are accessible as `v0` (for `ι`), `v1` (for `κ`), etc.
+Variables are accessible as `Typ.var 0` (for `ι`), `Typ.var 1` (for `κ`), etc.
 -/
 scoped macro "Π " κs:term,+ " ⇒ " body:term : term => do
-  κs.getElems.foldrM (fun arg body => `(Types.pi $arg $body)) body
+  κs.getElems.foldrM (fun arg body => `(Types.Typ.pi $arg $body)) body
 
-instance {Φ n} : OfNat (Types Φ .dim) n := ⟨.dim n⟩
+instance {n} : OfNat (Types.Typ) n := ⟨.dim n⟩
 
-instance {Φ} : Add (Types Φ .dim) where
-  add := Types.dimAdd
+instance : Add (Types.Typ) where
+  add := Types.Typ.dimAdd
 
-instance {Φ} : Append (Types Φ .shape) where
-  append := Types.shapeAppend
+instance : Append (Types.Typ) where
+  append := Types.Typ.shapeAppend
 
-scoped infix:50 " == " => Types.dimEq
+scoped infix:50 " == " => Types.Typ.dimEq
 
-open Lean in
-/--
-List syntax for `TList`s. Each kind has a special prefix to avoid syntax conflicts.
+/-!
+# Variable substitution in types
 -/
-def expandTList (ts : TSyntaxArray `term) (ι : TSyntax `term) : MacroM (TSyntax `term) := do
-  let nil : Lean.TSyntax `term ← `(TList.nil (κ := $ι))
-  let l ← ts.foldrM (fun hd tl => do return ← `(TList.cons ($hd) <| $tl)) nil
-  return l
 
-/-- Dimension list syntax: `d[1, 2, 3]` -/
-scoped macro "d[" ts:term,* "]" : term => do expandTList ts (← `(Kind.dim))
-/-- Shape list syntax: `s[shape1, shape2]` -/
-scoped macro "s[" ts:term,* "]" : term => do expandTList ts (← `(Kind.shape))
-/-- Type list syntax: `⋆[type1, type2]` -/
-scoped macro "⋆[" ts:term,* "]" : term => do expandTList ts (← `(Kind.type))
+/--
+`t[i := x]` substitutes `x` for the type variable with index `i` in `t`.
+-/
+macro:100 t:term "[" i:term " := " x:term "]" : term =>
+  `($(Lean.mkIdent `KLR.NKI.Types.Typ.subst) $x $i $t)
+
+/--
+`x.subst i t` substitutes `x` for the type variable with index `i` in `t`.
+
+We use the syntax `t[i := x] ≡ Typ.subst x i t`
+-/
+def Typ.subst (x : Typ) (i : Nat) : Typ → Typ
+  | var j => if i == j then x else var j
+  | pi κ typ => pi κ (typ[i + 1 := x])
+  | prim p => prim p
+  | func dom ran => func (dom[i := x]) (ran[i := x])
+  | dim n => dim n
+  | shape dims => shape (dims.map (·[i := x]))
+  | tensor sh dt => tensor (sh[i := x]) dt
+  | dimAdd d1 d2 => dimAdd (d1[i := x]) (d2[i := x])
+  | shapeAppend s1 s2 => shapeAppend (s1[i := x]) (s2[i := x])
+  | shapeTail s => shapeTail (s[i := x])
+
+@[app_unexpander Typ.subst]
+def unexpandTypSubst : Lean.PrettyPrinter.Unexpander
+  | `($_subst $x $i $t) => `(($t)[$i := $x])
+  | _ => throw ()
+-- #check Typ.subst (.prim .int) 0 (.var 0 ⟶ Π .typ ⇒ .var 0)
+-- #eval Typ.subst (.prim .int) 0 (.var 0 ⟶ Π .typ ⇒ .var 0)
+
+-- TODO: This notion of equivalence is too strong.
+-- We need to reason about equivalence of shapes constructed with operators, subtyping,
+-- and maybe α-equivalence
+def Typ.compat (t1 t2 : Typ) : Prop :=
+  t1 == t2
+
+instance Typ.instHasEquivTyp : HasEquiv Typ where
+  Equiv := Typ.compat
+
+instance Typ.decEquiv {t1 t2 : Typ} : Decidable (t1 ≈ t2) := by
+  simp only [HasEquiv.Equiv, compat]
+  cases t1 == t2
+  · apply isFalse; simp only [Bool.false_eq_true, not_false_eq_true]
+  · exact isTrue rfl
+
+/-!
+# Kind Checking for NKI Types
+-/
+
+abbrev TypCtx := List Kind
+
+/-- Context extension: `Φ,, κ ≡ κ :: Φ`. -/
+scoped notation Φ:70 ",, " κ:71 => @List.cons Kind κ Φ
+
+macro:65 Φ:term:70 " ⊢⋆ " α:term " : " κ:term : term =>
+  `($(Lean.mkIdent `KLR.NKI.Types.Typ.HasKind) $Φ $α $κ)
+
+inductive Typ.HasKind : TypCtx → Typ → Kind → Prop
+  | var {Φ : TypCtx} {κ : Kind}
+    (i : Nat) (h : Φ[i]? = κ) : Φ ⊢⋆ .var i : κ
+  | pi {Φ : TypCtx} {κ ι : Kind} {α : Typ}
+    : (Φ,, κ ⊢⋆ α : ι) → Φ ⊢⋆ .pi κ α : ι
+  | prim {Φ : TypCtx} {p : Prim} : Φ ⊢⋆ .prim p:⋆
+  | func {Φ : TypCtx} {dom ran : Typ}
+    : (Φ ⊢⋆ dom : ⋆) → (Φ ⊢⋆ ran : ⋆) → Φ ⊢⋆ dom ⟶ ran : ⋆
+  | dim {Φ : TypCtx} {n : Nat} : Φ ⊢⋆ .dim n : .dim
+  | shape {Φ : TypCtx} {dims : List Typ}
+    : (∀ dim ∈ dims, Φ ⊢⋆ dim : .dim) → Φ ⊢⋆ .shape dims : .shape
+  | tensor {Φ : TypCtx} {shape : Typ} {dt : Core.Dtype}
+    : (Φ ⊢⋆ shape : .shape) → Φ ⊢⋆ .tensor shape dt : ⋆
+  | dimAdd {Φ : TypCtx} {x y : Typ}
+    : (Φ ⊢⋆ x : .dim) → (Φ ⊢⋆ y : .dim) → Φ ⊢⋆ .dimAdd x y : .dim
+  | shapeAppend {Φ : TypCtx} {s1 s2 : Typ}
+    : (Φ ⊢⋆ s1 : .shape) → (Φ ⊢⋆ s2 : .shape) → Φ ⊢⋆ .shapeAppend s1 s2 : .shape
+  | shapeTail {Φ : TypCtx} {s : Typ}
+    : (Φ ⊢⋆ s : .shape) → Φ ⊢⋆ .shapeTail s : .shape
+
+@[app_unexpander Typ.HasKind]
+def unexpandHasKind : Lean.PrettyPrinter.Unexpander
+  | `($_HasKind $Φ $α $κ) => `($Φ ⊢⋆ $α : $κ)
+  | _ => throw ()
+
+/-!
+# Tactics for proving the decidability of kind-checking
+-/
+
+macro "dec_has_kind_cases" : tactic => `(tactic|(
+  case isFalse => exact isFalse fun h => by cases h; contradiction
+  case' isTrue =>
+    rename_i $(Lean.mkIdent `h):ident
+    try solve | (apply isTrue; constructor <;> try assumption)
+))
+
+macro "dec_has_kind_ih " Φ:term ", " α:term ", " κ:term : tactic => `(tactic|(
+  cases $(Lean.mkIdent `Typ.decHasKind) $Φ $α $κ
+  dec_has_kind_cases
+))
+
+macro "dec_has_kind_ih_list " Φ:term ", " αs:term ", " κ:term : tactic => `(tactic|(
+  cases $(Lean.mkIdent `Typ.listDecHasKind) $Φ $αs $κ
+  dec_has_kind_cases
+))
+
+macro "dec_has_kind_match_kind " κ:term ", " ι:term : tactic => `(tactic|(
+  by_cases $(Lean.mkIdent `heq):ident : $κ = $ι
+  case neg => exact isFalse fun h => by cases h; exact $(Lean.mkIdent `heq) rfl
+  case' pos =>
+    subst $(Lean.mkIdent `heq)
+    try solve | (apply isTrue; constructor <;> try assumption)
+))
+
+mutual
+
+instance Typ.listDecHasKind (Φ : TypCtx) (typs : List Typ) (κ : Kind) : Decidable (∀ α ∈ typs, Φ ⊢⋆ α : κ) :=
+  match typs with
+  | [] => isTrue fun _ h_mem => (List.not_mem_nil h_mem).elim
+  | hd :: tl =>
+    match Typ.decHasKind Φ hd κ with
+    | isTrue h =>
+      match Typ.listDecHasKind Φ tl κ with
+      | isTrue h => isTrue fun _ h_mem => by
+        simp_all only [List.mem_cons]
+        cases h_mem with
+        | inl h_2 =>
+          subst h_2
+          simp_all only
+        | inr h_3 => simp_all only
+      | isFalse hf => isFalse fun hf => by
+        simp_all only [List.mem_cons, true_or, or_true, implies_true, not_true_eq_false]
+    | isFalse hf =>
+      isFalse fun h =>
+        hf <| h hd (by
+          simp_all only [List.mem_cons, true_or, not_true_eq_false]
+        )
+
+/--
+Prove kind-checking of types is decidable
+-/
+instance Typ.decHasKind (Φ : TypCtx) (α : Typ) (κ : Kind) : Decidable (Φ ⊢⋆ α : κ) := by
+  match α with
+  | var i =>
+    match hm : Φ[i]? with
+    | some ι =>
+      if heq : κ = ι then
+        exact isTrue (.var i <| heq ▸ hm)
+      else
+        apply isFalse
+        intro h; cases h
+        simp_all only [Option.some.injEq]
+    | none =>
+      apply isFalse
+      intro h; cases h
+      simp_all only [reduceCtorEq]
+  | Π ι ⇒ β => dec_has_kind_ih (Φ,, ι), β, κ
+  | prim p => dec_has_kind_match_kind κ, ⋆
+  | func dom ran =>
+    dec_has_kind_match_kind κ, ⋆
+    case pos =>
+      dec_has_kind_ih Φ, dom, ⋆
+      dec_has_kind_ih Φ, ran, ⋆
+  | dim _ => dec_has_kind_match_kind κ, .dim
+  | shape dims =>
+    dec_has_kind_match_kind κ, .shape
+    case pos =>
+      dec_has_kind_ih_list Φ, dims, .dim
+  | tensor s dt =>
+    dec_has_kind_match_kind κ, ⋆
+    case pos =>
+      dec_has_kind_ih Φ, s, .shape
+  | dimAdd x y =>
+    dec_has_kind_match_kind κ, .dim
+    case pos =>
+      dec_has_kind_ih Φ, x, .dim
+      dec_has_kind_ih Φ, y, .dim
+  | shapeAppend s1 s2 =>
+    dec_has_kind_match_kind κ, .shape
+    case pos =>
+      dec_has_kind_ih Φ, s1, .shape
+      dec_has_kind_ih Φ, s2, .shape
+  | shapeTail s =>
+    dec_has_kind_match_kind κ, .shape
+    case pos =>
+      dec_has_kind_ih Φ, s, .shape
+
+end
+
+abbrev TypCheck := Compile.Pass.PosM Typ
+
+def Typ.reduceShape (Φ : TypCtx) : Typ → TypCheck
+  | .shape dims =>
+    if ∀ d ∈ dims, Φ ⊢⋆ d : .dim then
+      return .shape dims
+    else
+      throw "tensor dimension must have kind dim"
+  | .shapeAppend s1 s2 => do
+    let s1 ← s1.reduceShape Φ
+    let s2 ← s2.reduceShape Φ
+    match s1, s2 with
+    | .shape dims1, .shape dims2 => return .shape (dims1 ++ dims2)
+    | s1, s2 => return .shapeAppend s1 s2
+  | .shapeTail s => do
+    let s ← s.reduceShape Φ
+    match s with
+    | .shape [] => throw "cannot take the tail of an empty list of dimensions"
+    | .shape (_::tl) => return .shape tl
+    | s => return .shapeTail s
+  | s =>
+    if Φ ⊢⋆ s : .shape then
+      return s
+    else
+      throw "expected kind shape"
 
 namespace TypesExamples
+open Typ
 
 /--
 Matrix multiplication.
@@ -174,15 +372,19 @@ def matmul(x, y):
   """
 ```
 -/
-def matMul {Φ} (dtype : Core.Dtype) : Φ ⊢⋆ ⋆ :=
+def matMul (dtype : Core.Dtype) : Typ :=
   Π .dim, .dim, .dim ⇒
-    let M := v2
-    let N := v1
-    let K := v0
-    let x := .tensor (.shape d[M, N]) dtype
-    let y := .tensor (.shape d[N, K]) dtype
-    let out := .tensor (.shape d[M, K]) dtype
-    .tuple ⋆[x, y] → out
+    let M := var 2
+    let N := var 1
+    let K := var 0
+    let x := tensor (shape [M, N]) dtype
+    let y := tensor (shape [N, K]) dtype
+    let out := tensor (shape [M, K]) dtype
+    x ⟶ y ⟶ out
+
+example {Φ dtype} : Φ ⊢⋆ matMul dtype : ⋆ := by
+  apply of_decide_eq_true
+  rfl
 
 /--
 Batched matrix multiplication.
@@ -199,16 +401,20 @@ def batch_matmul(x, y):
   """
 ```
 -/
-def batchMatMul {Φ} (dtype : Core.Dtype) : Φ ⊢⋆ ⋆ :=
+def batchMatMul (dtype : Core.Dtype) : Typ :=
   Π .dim, .dim, .dim, .shape ⇒
-    let M := v3
-    let N := v2
-    let K := v1
-    let batch := v0
-    let x := .tensor (batch ++ (.shape d[M, N])) dtype
-    let y := .tensor (batch ++ (.shape d[N, K])) dtype
-    let out := .tensor (batch ++ (.shape d[M, K])) dtype
-    .tuple ⋆[x, y] → out
+    let M := var 3
+    let N := var 2
+    let K := var 1
+    let batch := var 0
+    let x := tensor (batch ++ (shape [M, N])) dtype
+    let y := tensor (batch ++ (shape [N, K])) dtype
+    let out := tensor (batch ++ (shape [M, K])) dtype
+    x ⟶ y ⟶ out
+
+example {Φ dtype} : Φ ⊢⋆ batchMatMul dtype : ⋆ := by
+  apply of_decide_eq_true
+  rfl
 
 /--
 Concatenation along the last axis.
@@ -225,16 +431,16 @@ def concat_last_axis(x, y):
   """
 ```
 -/
-def concatLastAxis {Φ} (dtype : Core.Dtype) : Φ ⊢⋆ ⋆ :=
+def concatLastAxis (dtype : Core.Dtype) : Typ :=
   Π .dim, .dim, .shape ⇒
-    let M := v2
-    let N := v1
-    let shape := v0
-    let x := .tensor (shape ++ (.shape d[M])) dtype
-    let y := .tensor (shape ++ (.shape d[N])) dtype
-    let out := .tensor (shape ++ (.shape d[M + N])) dtype
-    .tuple ⋆[x, y] → out
+    let M := var 2
+    let N := var 1
+    let s := var 0
+    let x := tensor (s ++ (shape [M])) dtype
+    let y := tensor (s ++ (shape [N])) dtype
+    let out := tensor (s ++ (shape [M + N])) dtype
+    x ⟶ y ⟶ out
 
-end TypesExamples
-
-end KLR.NKI.Types
+example {Φ dtype} : Φ ⊢⋆ concatLastAxis dtype : ⋆ := by
+  apply of_decide_eq_true
+  rfl
