KLR/NKI/TIR.lean
@@ -1,0 +1,376 @@
+/-
+Copyright (c) 2025 Amazon.com, Inc. or its affiliates. All Rights Reserved.
+Released under Apache 2.0 license as described in the file LICENSE.
+Authors: Paul Mure
+-/
+import KLR.NKI.Simplify
+import KLR.NKI.Types
+import KLR.Compile.Pass
+
+/-!
+# Typed IR for NKI
+
+This includes the following simplications
+- Tuples are removed
+- Function calls are curried and no default or keyword args are allowed
+- Binnary ops become calls of constant functions
+- `Stmt`s have `seq` which removed the need for `List Stmt`
+- Introduce let bindings in `Stmt`
+- No un-initialized variables allowed
+-/
+
+namespace KLR.NKI
+
+namespace TIR
+
+inductive Value where
+  | none
+  | bool (value : Bool)
+  | int (value : Int)
+  | float (value : Float)
+  | string (value : String)
+  | tensor (shape : List Nat) (dtype : Core.Dtype) --(value : TensorLib.Tensor)
+
+/--
+TODO: Manage overloading better?
+-/
+inductive Const where
+  -- logical
+  | land | lor
+  -- bitwise
+  | lshift | rshift | or | xor | and
+  -- comparison
+  | eq | ne
+  | lt_int_int | lt_int_float | lt_float_int | lt_float_float
+  | le_int_int | le_int_float | le_float_int | le_float_float
+  | gt_int_int | gt_int_float | gt_float_int | gt_float_float
+  | ge_int_int | ge_int_float | ge_float_int | ge_float_float
+  -- arithmetic
+  | add_int_int | add_int_float | add_float_int | add_float_float
+  | sub_int_int | sub_int_float | sub_float_int | sub_float_float
+  | mul_int_int | mul_int_float | mul_float_int | mul_float_float
+  | div_int_int | div_int_float | div_float_int | div_float_float
+  | mod_int_int | mod_int_float | mod_float_int | mod_float_float
+  | pow_int_int  | pow_int_float | pow_float_int | pow_float_float
+  | floor_int_int | floor_int_float | floor_float_int | floor_float_float
+
+mutual
+
+inductive Index where
+  | coord (i : Expr)
+  | slice (l u step : Option Expr)
+  | ellipsis
+
+structure Expr where
+  expr : Expr'
+  pos : Pos
+
+inductive Expr' where
+  | const (const : Const)
+  | value (value : Value)
+  | var (name : String)
+  | access (expr : Expr) (indices : List Index)
+  | ifExp (test body orelse : Expr)
+  | app (f : Expr) (arg : Expr)
+  | typApp (f : Expr) (arg : Types.Typ)
+
+end
+
+mutual
+
+structure Stmt where
+  stmt : Stmt'
+  pos : Pos
+
+inductive Stmt' where
+  | expr (e : Expr)
+  | ret (e : Expr)
+  | let_ (var : String) (ty : Types.Typ) (rhs : Expr) (body : Stmt)
+  | ifStm (e : Expr) (thn els : Stmt)
+  | forLoop (x : String) (iter : Expr) (body : Stmt)
+  | breakLoop
+  | continueLoop
+  | seq (s1 s2 : Stmt)
+
+end
+
+structure Fun where
+  name : String
+  file : String
+  line : Nat
+  body : Stmt
+  typArgs : List Types.Kind
+  argNames : List String
+  argTyps : List Types.Typ
+  retTyp : Types.Typ
+
+structure Arg where
+  name : String
+  value : Expr
+  typ : Types.Typ
+
+structure Kernel where
+  entry : String
+  typArgs : List Types.Typ
+  args : List Expr
+  funs : List Fun
+  globals : List Arg
+
+def mkKernelApp (entry : String) (typArgs : List Types.Typ) (args : List Expr) : Expr :=
+  let pos : Pos := ⟨0, 0, none, none⟩ -- TODO: what pos to use here?
+  let typApp := typArgs.foldl (fun res typ => ⟨.typApp res typ, pos⟩) ⟨.var entry, pos⟩
+  args.foldl (fun res arg => ⟨.app res arg, pos⟩) typApp
+
+/-!
+# Typing Rules
+-/
+open Types Compile.Pass
+
+def Fun.sig (f : Fun) : Typ :=
+  f.typArgs.foldr (fun κ typ => Π κ ⇒ typ)
+  <| f.argTyps.foldr (fun argTyp retTyp => argTyp ⟶ retTyp) f.retTyp
+
+structure Ctx where
+  typs : TypCtx
+  vars : List (String × Typ)
+  retTyp : Option Typ
+
+def Ctx.empty : Ctx :=
+  ⟨[], [], none⟩
+
+/--
+  Set the type of the variable with `name` to be `typ`
+-/
+def Ctx.updateVar (Γ : Ctx) (name : String) (typ : Typ) : Ctx :=
+  let vars := (name, typ) :: Γ.vars.filter (·.1 == name)
+  {Γ with vars := vars}
+
+def Ctx.updateVars (Γ : Ctx) (vars : List (String × Typ)) : Ctx :=
+  vars.foldl (fun Γ (name, typ) => Γ.updateVar name typ) Γ
+
+def Ctx.addTyp (Γ : Ctx) (κ : Kind) : Ctx :=
+  {Γ with typs := Γ.typs,, κ}
+
+def Ctx.setRet (Γ : Ctx) (ret : Typ) : Ctx :=
+  {Γ with retTyp := some ret}
+
+def Ctx.kernelInit (globals : List Arg) (funs : List Fun) : Ctx :=
+  let globals := globals.map fun arg => (arg.name, arg.typ)
+  let funVars := funs.map fun f => (f.name, f.sig)
+  Ctx.empty.updateVars (globals ++ funVars)
+
+def Ctx.addTyps (Γ : Ctx) (κs : List Kind) : Ctx :=
+  {Γ with typs := Γ.typs ++ κs}
+
+def Ctx.enterFun (Γ : Ctx) (typArgs : List Kind) (argNames : List String) (argTyps : List Typ) (retTyp : Typ) : Ctx :=
+  ((Γ.addTyps typArgs).updateVars (argNames.zip argTyps)).setRet retTyp
+
+def Ctx.addFun (Γ : Ctx) (f : Fun) : Ctx :=
+  Γ.updateVar f.name f.sig
+
+def Ctx.addFuns (Γ : Ctx) (funs : List Fun) : Ctx :=
+  funs.foldl (fun Γ f => Γ.addFun f) Γ
+
+/-!
+# Type checking functions
+-/
+
+def Value.typ : Value → Typ
+  | .none => .prim .none
+  | .bool _ => .prim .bool
+  | .int _ => .prim .int
+  | .float _ => .prim .float
+  | .string _ => .prim .string
+  | .tensor shape dtype => .tensor (.shape <| shape.map .dim) dtype
+
+def Const.typ : Const → Typ
+  -- logical
+  | .land => .prim .bool ⟶ .prim .bool ⟶ .prim .bool
+  | .lor => .prim .bool ⟶ .prim .bool ⟶ .prim .bool
+  -- bitwise
+  | .lshift => .prim .int ⟶ .prim .int ⟶ .prim .int
+  | .rshift => .prim .int ⟶ .prim .int ⟶ .prim .int
+  | .or => .prim .int ⟶ .prim .int ⟶ .prim .int
+  | .xor => .prim .int ⟶ .prim .int ⟶ .prim .int
+  | .and => .prim .int ⟶ .prim .int ⟶ .prim .int
+  -- comparison
+  | .eq => Π ⋆ ⇒ .var 0 ⟶ .var 0 ⟶ .prim .bool
+  | .ne => Π ⋆ ⇒ .var 0 ⟶ .var 0 ⟶ .prim .bool
+  | .lt_int_int => .prim .int ⟶ .prim .int ⟶ .prim .bool
+  | .lt_int_float => .prim .int ⟶ .prim .float ⟶ .prim .bool
+  | .lt_float_int => .prim .float ⟶ .prim .int ⟶ .prim .bool
+  | .lt_float_float => .prim .float ⟶ .prim .float ⟶ .prim .bool
+  | .le_int_int => .prim .int ⟶ .prim .int ⟶ .prim .bool
+  | .le_int_float => .prim .int ⟶ .prim .float ⟶ .prim .bool
+  | .le_float_int => .prim .float ⟶ .prim .int ⟶ .prim .bool
+  | .le_float_float => .prim .float ⟶ .prim .float ⟶ .prim .bool
+  | .gt_int_int => .prim .int ⟶ .prim .int ⟶ .prim .bool
+  | .gt_int_float => .prim .int ⟶ .prim .float ⟶ .prim .bool
+  | .gt_float_int => .prim .float ⟶ .prim .int ⟶ .prim .bool
+  | .gt_float_float => .prim .float ⟶ .prim .float ⟶ .prim .bool
+  | .ge_int_int => .prim .int ⟶ .prim .int ⟶ .prim .bool
+  | .ge_int_float => .prim .int ⟶ .prim .float ⟶ .prim .bool
+  | .ge_float_int => .prim .float ⟶ .prim .int ⟶ .prim .bool
+  | .ge_float_float => .prim .float ⟶ .prim .float ⟶ .prim .bool
+  -- arithmetic
+  | .add_int_int => .prim .int ⟶ .prim .int ⟶ .prim .int
+  | .add_int_float => .prim .int ⟶ .prim .float ⟶ .prim .float
+  | .add_float_int => .prim .float ⟶ .prim .int ⟶ .prim .float
+  | .add_float_float => .prim .float ⟶ .prim .float ⟶ .prim .float
+  | .sub_int_int => .prim .int ⟶ .prim .int ⟶ .prim .int
+  | .sub_int_float => .prim .int ⟶ .prim .float ⟶ .prim .float
+  | .sub_float_int => .prim .float ⟶ .prim .int ⟶ .prim .float
+  | .sub_float_float => .prim .float ⟶ .prim .float ⟶ .prim .float
+  | .mul_int_int => .prim .int ⟶ .prim .int ⟶ .prim .int
+  | .mul_int_float => .prim .int ⟶ .prim .float ⟶ .prim .float
+  | .mul_float_int => .prim .float ⟶ .prim .int ⟶ .prim .float
+  | .mul_float_float => .prim .float ⟶ .prim .float ⟶ .prim .float
+  | .div_int_int => .prim .int ⟶ .prim .int ⟶ .prim .int
+  | .div_int_float => .prim .int ⟶ .prim .float ⟶ .prim .float
+  | .div_float_int => .prim .float ⟶ .prim .int ⟶ .prim .float
+  | .div_float_float => .prim .float ⟶ .prim .float ⟶ .prim .float
+  | .mod_int_int => .prim .int ⟶ .prim .int ⟶ .prim .int
+  | .mod_int_float => .prim .int ⟶ .prim .float ⟶ .prim .float
+  | .mod_float_int => .prim .float ⟶ .prim .int ⟶ .prim .float
+  | .mod_float_float => .prim .float ⟶ .prim .float ⟶ .prim .float
+  | .pow_int_int => .prim .int ⟶ .prim .int ⟶ .prim .int
+  | .pow_int_float => .prim .int ⟶ .prim .float ⟶ .prim .float
+  | .pow_float_int => .prim .float ⟶ .prim .int ⟶ .prim .float
+  | .pow_float_float => .prim .float ⟶ .prim .float ⟶ .prim .float
+  | .floor_int_int => .prim .int ⟶ .prim .int ⟶ .prim .int
+  | .floor_int_float => .prim .int ⟶ .prim .float ⟶ .prim .float
+  | .floor_float_int => .prim .float ⟶ .prim .int ⟶ .prim .float
+  | .floor_float_float => .prim .float ⟶ .prim .float ⟶ .prim .float
+
+inductive IndexKind
+  | coord
+  | slice
+  | ellipsis
+
+mutual
+
+def Option.hasIntTyp (Γ : Ctx) : Option Expr → PosM Unit
+  | some e => do
+    let .prim .int ← e.typ Γ | throw "expected type int"
+  | none => none
+
+def Index.kind (Γ : Ctx) : Index → PosM IndexKind
+  | .coord i => do
+    let .prim .int ← i.typ Γ | throw "tensor index must be of type int"
+    return .coord
+  | .slice l u step => do
+    let _ ← Option.hasIntTyp Γ l
+    let _ ← Option.hasIntTyp Γ u
+    let _ ← Option.hasIntTyp Γ step
+    return .slice
+  | .ellipsis => return .ellipsis
+
+def Index.accessTyp (Γ : Ctx) (shape : Typ) (dtype : Core.Dtype) (indices : List IndexKind) : TypCheck := do
+  match (← shape.reduceShape Γ.typs), indices with
+  | .shape [_], [.coord] =>
+    return .prim (.dtype dtype)
+  | .shape (_::tl), [.coord] =>
+    return .tensor (.shape tl) dtype
+  | .shape (_::tl), .coord :: idxTl =>
+    Index.accessTyp Γ (.shape tl) dtype idxTl
+  | _, _ =>
+    throw "unsupported access pattern"
+
+def Expr.typ (Γ : Ctx) : Expr → TypCheck
+  | {expr, pos} => withPos pos do expr.typ Γ
+
+def Expr'.typ (Γ : Ctx) : Expr' → TypCheck
+  | .const const => return const.typ
+  | .value value => return value.typ
+  | .var name => do
+    let some (_, typ) := Γ.vars.find? (·.1 == name)
+      | throw s!"\"{name}\" not found in type context"
+    return typ
+  | .access expr indices => do
+    let .tensor shape dtype ← expr.typ Γ
+      | throw "only tensor access is currently supported"
+    let indices ← indices.mapM (Index.kind Γ)
+    Index.accessTyp Γ shape dtype indices
+  | .ifExp test body orelse => do
+    let .prim .bool ← test.typ Γ
+      | throw "condition of an if-expression must have type bool"
+    let tBody ← body.typ Γ
+    let tOrelse ← orelse.typ Γ
+    if tBody ≈ tOrelse then
+      return tBody
+    else
+      throw "both branches of an if-expression must have the same type"
+  | .app f arg => do
+    let dom ⟶ ran ← f.typ Γ
+      | throw "only functions can be applied"
+    let argTyp ← arg.typ Γ
+    if dom ≈ argTyp then -- TODO: subtyping
+      return ran
+    else
+      throw "argument type mismatch"
+  | .typApp f arg => do
+    let Π κ ⇒ t ← f.typ Γ
+      | throw "invalid polymorphic instantiation"
+    if Γ.typs ⊢⋆ arg : κ then
+      return t[0 := arg]
+    else
+      throw "argument kind mismatch"
+
+end
+
+mutual
+
+def Stmt.typ (Γ : Ctx) : Stmt → TypCheck
+  | { stmt, pos } => withPos pos do stmt.typ Γ
+
+def Stmt'.typ (Γ : Ctx) : Stmt' → TypCheck
+  | .expr e => e.typ Γ
+  | .ret e => do
+    let t ← e.typ Γ
+    let some expected := Γ.retTyp
+      | throw "return outside of a a function"
+    if t ≈ expected then -- TODO: subtyping
+      return expected
+    else
+      throw "return type mismatch"
+  | .let_ var ty rhs body => do
+    let t ← rhs.typ Γ
+    if t ≈ ty then -- TODO: subtyping
+      body.typ (Γ.updateVar var ty)
+    else
+      throw "type mismatch"
+  | .ifStm e thn els => do
+    let .prim .bool ← e.typ Γ
+      | throw "condition of if statement must be bool"
+    let _ ← thn.typ Γ
+    let _ ← els.typ Γ
+    return .prim .none
+  | .forLoop _ _ _ =>
+    -- TODO
+    throw "forLoop not currently supported"
+  | .breakLoop => return .prim .none
+  | .continueLoop => return .prim .none
+  | .seq s1 s2 => do
+    let _ ← s1.typ Γ
+    s2.typ Γ
+
+end
+
+def Fun.typ (Γ : Ctx) (f : Fun) : TypCheck := do
+  let ret ← f.body.typ (Γ.enterFun f.typArgs f.argNames f.argTyps f.retTyp)
+  if ret ≈ f.retTyp then -- TODO: subtyping
+    return f.sig
+  else
+    throw "function return type mismatch"
+
+def Kernel.typ (k : Kernel) : TypCheck := do
+  let _ ← List.mapM (fun arg => do
+    let typ ← arg.value.typ .empty
+    if typ ≈ arg.typ then -- TODO: subtyping
+      return
+    else
+      throw "global arg type mismatch"
+  ) k.globals
+  let Γ := Ctx.kernelInit k.globals k.funs
+  let _ ← List.mapM (Fun.typ Γ) k.funs
+  (mkKernelApp k.entry k.typArgs k.args).typ Γ
